totally rework fields, move to typeclasses per field rather than fin and Coq's pattern matching. Not sure how well the typeclass resolution will work with cleaner syntax.

RGref/DSL/Fields.v
@@ -2,27 +2,27 @@ Require Import RGref.DSL.DSL.
 Require Import Coq.Vectors.Fin.
 Require Import Coq.Arith.Arith.
 
-Definition fin := t. (* Why on earth is this named t in the stdlib??? *)
+(* Field Typing is a tagging mechanism, that fields of T are indexed by F *)
+Class FieldTyping (T : Set) (F : Set) : Set := {}.
 
-Definition FieldTypes (n : nat) := fin n -> Set.
-
-Class FieldAccess (T : Set) {n : nat} (ft : FieldTypes n) : Set := {
-  fieldOf : forall (obj : T) (x : fin n), ft x ;
-  fieldUpdate : forall (obj : T) (x : fin n) (v : ft x), T
+Class FieldType (T : Set) (F : Set) `{FieldTyping T F} (f:F) (FT : Set) := {
+  getF : T -> FT;
+  setF : T -> FT -> T
+  (* In theory we could also require a proof that it satisfies the theory
+     of arrays, e.g. forall x v, getF (setF x v) = v. *)
 }.
 
 (* Field-aware heap access primitives *)
-Axiom field_read : forall {T B Res:Set}{P R G}{n:nat}{ft:FieldTypes n}`{rel_fold T}
+Axiom field_read : forall {T B F Res:Set}{P R G}`{rel_fold T}
                           `{rgfold R G = B}
                           `{hreflexive G}
-                          `{FieldAccess B n ft}
-                          (r:ref{T|P}[R,G]) (f:fin n)
-                          `{ft f = Res}, (* <-- another weak pattern matching/conversion hack *)
+                          (r:ref{T|P}[R,G]) (f:F)
+                          `{FieldType B F f Res},
                           Res.
-Axiom field_write : forall {Γ}{T:Set}{P R G}{n:nat}{ft:FieldTypes n}
-                           `{FieldAccess T n ft}
-                           (r:ref{T|P}[R,G]) (f:fin n) (e : ft f)
-                           `{forall h v, P v h -> G v (fieldUpdate v f e) h (heap_write r (fieldUpdate v f e) h)},
+Axiom field_write : forall {Γ}{T F Res:Set}{P R G}
+                           (r:ref{T|P}[R,G]) (f:F) (e : Res)
+                           `{FieldType T F f Res}
+                           `{forall h v, P v h -> G v (setF v e) h (heap_write r (setF v e) h)},
                            rgref Γ unit Γ.
 
 Section FieldDemo.
@@ -35,64 +35,25 @@ Section FieldDemo.
   Lemma refl_deltaD : hreflexive deltaD. Proof. red. intros. destruct x. apply incCount. eauto with arith. Qed.
   Hint Resolve refl_deltaD.
 
-  (* This demonstrates why Fin is more heavily used in Agda than Coq.
-     Coq's pattern matching is too weak to determine that F1 and FS _ (F1 _)
-     is an exhaustive match! *)
-  Definition DFieldSize := FieldTypes 2.
-  Definition DFieldTypes : FieldTypes 2 :=
-    fun f => match f as F with
-             | F1 _ => nat
-             | FS _ _ => bool
-             end. 
   Inductive Dfield : Set := Count | Flag.
-  Definition DField2Fin (df : Dfield) : fin 2 := match df with Count => F1 | Flag => FS (F1) end.
-  Coercion DField2Fin : Dfield >-> fin.
-  Require Import Coq.Program.Equality. (* dependent induction tactic *)
-  (* More hacks for weak conversion and pattern matching... *)
-  Definition nat2DField (n : nat) : DFieldTypes Count. compute; assumption. Defined.
-  Definition nat2DField' (n : nat) : DFieldTypes (@F1 (S O)). compute; assumption. Defined.
-  Definition Count2nat (n : DFieldTypes Count) : nat. compute; assumption. Defined.
-  Definition bool2DField (b : bool) : DFieldTypes Flag. compute; assumption. Defined.
-  Print nat2DField'.
+  Instance dfields : FieldTyping D Dfield.
+  Instance dfield_count : FieldType D Dfield Count nat := {
+    getF := fun v => match v with (mkD n b) => n end;
+    setF := fun v fv => match v with (mkD n b) => (mkD fv b) end
+  }.
+  Instance dfield_flag : FieldType D Dfield Flag bool := {
+    getF := fun v => match v with (mkD n b) => b end;
+    setF := fun v fv => match v with (mkD n b) => (mkD n fv) end
+  }.
+
   Definition getCount (d:D) := match d with (mkD n b) => n end.
   Definition getFlag (d:D) := match d with (mkD n b) => b end.
-  Program Instance DAccess : FieldAccess D DFieldTypes :=
-(* Ideally we'd just directly define, but Coq's pattern matching is weak, so we'll use the refine tactic. :=*)
-  { fieldOf := fun obj x => (*match obj with (mkD n b) =>
-                              match x as x in t _ return DFieldTypes _ with
-                              | F1 f1n => _
-                              | FS fsn finB => _
-                              end
-                            end;*)
-(*                            match x as y return (x = y -> DFieldTypes x) with*)
-                            match x as y return DFieldTypes x with
-                            | F1 f1n => _
-                            | FS fsn finB => _
-                            end ;
 
-    fieldUpdate := fun obj f v =>
-                     match obj with (mkD n b) =>
-                       match f as f return D with
-                         | (F1 f1n) =>  mkD (_ n) b 
-                         | (FS fsn finB) => mkD n (_ b)
-                       end
-                     end
-  }.
-  Next Obligation. compute. induction x. refine (getCount obj). refine (getFlag obj). Defined. 
-  Next Obligation. compute. induction x. refine (getCount obj). refine (getFlag obj). Defined.
-
-Print DAccess.
-(*
-  constructor. 
-  (* fieldOf *) intro obj. intro x. destruct obj.
-                dependent induction x; red; auto.
-  (* fieldUpdate *) intros obj x v. destruct obj.
-                    dependent induction x; compute [DFieldTypes] in *. exact (mkD v b). exact (mkD n v).
-  Defined.*)
 (* Print DAccess. (* <-- that is a terrible term due to dependent induction *) *)
   Instance pureD : pure_type D.
   Program Example demo {Γ} (r : ref{D|any}[deltaD,deltaD]) : rgref Γ unit Γ :=
-    @field_write Γ D _ _ _ _ _ DAccess r Count (nat2DField ((Count2nat (@field_read _ _ _ _ _ _ _ _ _ _ _ DAccess r (DField2Fin Count) _)) + 1)) _.
+    @field_write Γ D Dfield nat _ _ _ r Count ((@field_read _ D Dfield _ _ _ _ _ _ _ r Count _ _)+1) _ _ _.
+(*    @field_write Γ D _ _ _ _ _ DAccess r Count (nat2DField ((Count2nat (@field_read _ _ _ _ _ _ _ _ _ _ _ DAccess r (DField2Fin Count) _)) + 1)) _.
   Next Obligation.
     cut (forall f p1 p2 p3, @eq (DFieldTypes f) (@field_read D D _ _ _ _ _ DFieldTypes _ p1 p2 DAccess r f p3)  (@fieldOf D _ DFieldTypes DAccess (@fold D _ deltaD deltaD v) f)).
     intro Hcomp. rewrite Hcomp with (f := F1).
@@ -107,5 +68,19 @@ Print DAccess.
     (* At this point we *should* be done, but the use of dependent induction to work around
        Coq's pattern matching has introduced some uses of JMeq to deal with *)
     generalize (@JMeq_eq (t (S (S O))) (@F1 (S O)) (@F1 (S O)) (@JMeq_refl (t (S (S O))) (@F1 (S O)))).
-    intro e. elim e.
+    intro e. elim e.*)
+
+  Next Obligation. unfold demo_obligation_1. unfold demo_obligation_2.
+    Check @getF.
+    cut (forall P R G pf1 pf2 r f fs fi, 
+           @field_read D D Dfield nat P R G (@pure_fold D pureD) pf1 pf2 r f fs fi = 
+                     @getF D Dfield _ f nat _ v).
+    intros Hfieldstuff.
+    destruct v.
+    rewrite Hfieldstuff.
+    compute. fold plus. constructor. eauto with arith.
+    (* this should be abstracted to a general hypothesis supplied by
+       the write framework. *)
+    admit.
+  Qed.
 End FieldDemo.
